value typing restructures; ctx interpreter progress

theories/typing.v
@@ -51,28 +51,28 @@ Definition ext_typing (s: store_record) (v: extern_value) : option extern_type :
 (** std-doc:
 For the purpose of checking argument values against the parameter types of exported functions, values are classified by value types. The following auxiliary typing rules specify this typing relation relative to a store S in which possibly referenced addresses live.
  **)
-Definition value_num_typing (s: store_record) (v: value_num) : value_type :=
-  T_num (typeof_num v).
+Definition value_num_typing (s: store_record) (v: value_num) : number_type :=
+  typeof_num v.
 
-Definition value_vec_typing (s: store_record) (v: value_vec) : value_type :=
-  T_vec (typeof_vec v).
+Definition value_vec_typing (s: store_record) (v: value_vec) : vector_type :=
+  typeof_vec v.
 
-Definition value_ref_typing (s: store_record) (v: value_ref) : option value_type :=
+Definition value_ref_typing (s: store_record) (v: value_ref) : option reference_type :=
   match v with
-  | VAL_ref_null t => Some (T_ref t)
+  | VAL_ref_null t => Some t
   | VAL_ref_func addr =>
       match ext_func_typing s addr with
-      | Some ft => Some (T_ref T_funcref)
+      | Some ft => Some T_funcref
       | _ => None
       end
-  | VAL_ref_extern eaddr => Some (T_ref T_externref)
+  | VAL_ref_extern eaddr => Some T_externref
   end.
 
 Definition value_typing (s: store_record) (v: value) : option value_type :=
   match v with
-  | VAL_num v' => Some (value_num_typing s v')
-  | VAL_vec v' => Some (value_vec_typing s v')
-  | VAL_ref v' => value_ref_typing s v'
+  | VAL_num v' => Some (T_num (value_num_typing s v'))
+  | VAL_vec v' => Some (T_vec (value_vec_typing s v'))
+  | VAL_ref v' => option_map T_ref (value_ref_typing s v')
   end.                      
 
 Definition values_typing (s: store_record) (vs: list value) : option (list value_type) :=
@@ -457,7 +457,7 @@ Definition tableinst_typing (s: store_record) (ti: tableinst) : option table_typ
   let '{| tableinst_type := ti_type; tableinst_elem := refs |} := ti in
   if tabletype_valid ti_type then
     if length refs == ti_type.(tt_limits).(lim_min) then
-      if all (fun ref => (value_ref_typing s ref == Some (T_ref (ti_type.(tt_elem_type))))) refs then
+      if all (fun ref => (value_ref_typing s ref == Some (ti_type.(tt_elem_type)))) refs then
         Some ti_type
       else None
     else None
@@ -481,7 +481,7 @@ Definition globalinst_typing (s: store_record) (gi: globalinst) : option global_
 
 Definition eleminst_typing (s: store_record) (ei: eleminst) : option reference_type :=
   let '{| eleminst_type := ei_type; eleminst_elem := refs |} := ei in
-  if all (fun ref => (value_ref_typing s ref == Some (T_ref ei_type))) refs then
+  if all (fun ref => (value_ref_typing s ref == Some ei_type)) refs then
     Some ei_type
   else None.
 
